\documentclass{report}
    \linespread{1.5}
    
    \usepackage{amsmath}
    \usepackage{amssymb}
    
    
    \begin{document}
    CISC102 - Discrete Math I

    July 2018

    \bigskip
    
    Assignment 3 - Problem 3
    
    Sam Huang (10175794)
    \bigskip
    
    
    \centerline{\textbf{Prove that}}
    
    $\forall n \geq 1$, 
    
    $\frac{1}{1*2}$ + $\frac{1}{2*3}$ + $\frac{1}{3*4}$ + ... + $\frac{1}{n(n+1)}$ = $\frac{n}{n+1}$
    
    \bigskip
    \bigskip
    
    \centerline{\textbf{Proof by induction}}
     
    \underline{Base Case}: n = 1
    
    $\rightarrow \frac{1}{1(1+1)}$ = $\frac{1}{1+1}$
    
    $\rightarrow \frac{1}{2}$ = $\frac{1}{2}$
    
    \medskip
    
    $\therefore LHS = RHS \implies$ the statement is true for the Base Case
    
    \bigskip
    
    \underline{Inductive Hypothesis}: Assume the statement is true for some integer $k \geq 1$
    
    That is, $\frac{1}{1*2}$ + $\frac{1}{2*3}$ + $\frac{1}{3*4}$ + ... + $\frac{1}{k(k+1)}$ = $\frac{k}{k+1}$
    
    \medskip
    
    Now consider the case where n = k+1 (the next integer) 
    
    $\frac{1}{1*2}$ + $\frac{1}{2*3}$ + $\frac{1}{3*4}$ + ... + $\frac{1}{k(k+1)}$ + $\frac{1}{(k+1)(k+1+1)}$ = $\frac{k+1}{k+1+1}$
    
    \medskip
    
    $\rightarrow (\frac{1}{1*2}$ + $\frac{1}{2*3}$ + $\frac{1}{3*4}$ + ... + $\frac{1}{k(k+1)}$) + $\frac{1}{(k+1)(k+2)}$ = $\frac{k+1}{k+2}$
    
    \textit{Here we can substitute the inductive hypothesis for the bracketed section}
    
    $\rightarrow \frac{k}{k+1}$ + $\frac{1}{(k+1)(k+2)}$ = $\frac{k+1}{k+2}$
    
    \textit{Multiply both sides by (k+1)(k+2)}
    
    $\rightarrow k(k+2) + 1 = (k+1)(k+1)$
    
    \textit{Expand}
    
    $\rightarrow k^{2} +2k + 1 = k^{2} +k +k +1^{2}$
    
    \textit{Simplify}
    
    $\rightarrow k^{2} +2k + 1 = k^{2} + 2k + 1$
    
    $\therefore LHS = RHS \implies$ the Inductive Hypothesis is true
    
    \bigskip
    
    Putting the Base Case and the Inductive Hypothesis together, we conclude 
    
    that the statement $\frac{1}{1*2}$ + $\frac{1}{2*3}$ + $\frac{1}{3*4}$ + ... + $\frac{1}{n(n+1)}$ = $\frac{n}{n+1}$ is true, $\forall n \geq 1$
    $\blacksquare$ 
    
    \end{document}
    
    